float_test6.bpl
@@ -1,5 +1,40 @@
-procedure F() returns () {
-	var x : float;
-	var y : float;
-	assert (x + x) + (y + y) == fp(0);
+//Translation from filter2.c
+//Should give an error
+//FAILS; doesn't generate terms!
+
+procedure main() returns () {
+	var E : float(11 53);
+	var E0 : float(11 53);
+	var E1 : float(11 53);
+	var S : float(11 53);
+	var S0 : float(11 53);
+	var S1 : float(11 53);
+	var i: int;
+	
+	havoc E;
+	havoc E0;
+	assume(E >= fp(0.0 11 53) && E <= fp(1.0 11 53));
+	assume(E0 >= fp(0.0 11 53) && E0 <= fp(1.0 11 53));
+	
+	E1 := fp(0.0 11 53);
+	S1 := fp(0.0 11 53);
+	S0 := fp(0.0 11 53);
+	S := fp(0.0 11 53);
+	
+	i := 0;
+//	while (i <= 1000000)
+//	{
+		E1 := E0;
+		E0 := E;
+	
+		havoc E;
+		assume(E >= fp(0.0 11 53) && E <= fp(1.0 11 53));
+		
+		S1 := S0;
+		S0 := S;
+		S := E*fp(0.7 11 53) - E0*fp(1.3 11 53) + E1*fp(1.1 11 53) + S0*fp(1.4 11 53) - S1*fp(0.7 11 53);
+		
+		assert(S >= fp(-4.0 11 53) && S <= fp(4.0 11 53));
+		//i := i + 1;
+//	}
 }
