float_test7.bpl
@@ -1,5 +1,38 @@
-procedure F() returns () {
-	var x : float;
-	x := fp(.1) + fp(.1) + fp(.1);
-	assert x == fp(.3);
+//Translation from filter2.c
+//Should give an error
+//Same as the previous one; it works with reals!
+
+procedure main() returns () {
+	var E : real;
+	var E0 : real;
+	var E1 : real;
+	var S : real;
+	var S0 : real;
+	var S1 : real;
+	var i: int;
+	
+	havoc E;
+	havoc E0;
+	assume(E >= 0.0 && E <= 1.0);
+	assume(E0 >= 0.0 && E0 <= 1.0);
+	
+	S0 := 0.0;
+	S := 0.0;
+	
+	i := 0;
+	while (i <= 1000000)
+	{
+		E1 := E0;
+		E0 := E;
+		
+		havoc E;
+		assume(E >= 0.0 && E <= 1.0);
+		
+		S1 := S0;
+		S0 := S;
+		S := E*0.7 - E0*1.3 + E1*1.1 + S0*1.4 - S1*0.7;
+		
+		assert(S >= -4.0 && S <= 4.0);
+		i := i + 1;
+	}
 }
