float_test.bpl
@@ -1,5 +1,13 @@
-procedure F(n: float) returns(r: float)
-	ensures r == n;
-{
-	r := n;
+//Translation from addsub_double_exact.c
+//Should Verify
+procedure main() returns () {
+	var x : float(11 53);
+	var y : float(11 53);
+	var z : float(11 53);
+	var r : float(11 53);
+	x := fp(10000000 11 53);
+	y := x + fp(1 11 53);
+	z := x - fp(1 11 53);
+	r := y - z;
+	assert r == fp(2 11 53);
 }
