float_test14.bpl
@@ -1,0 +1,17 @@
+//Translation from inv_square_false-unreach-call.c
+//Should Verify
+
+procedure main() returns () {
+	var x : float;
+	var y : float;
+	var z : float;
+	
+	havoc x;
+	assume(x >= fp(-1) && x <= fp(1));
+	
+	if (x <= fp(-.00000000000000000001) || x >= fp(.00000000000000000001)) {
+		y := x * x;
+		assert(y != fp(0));
+		z := fp(1) / y;
+	}
+}
