float_test15.bpl
@@ -1,0 +1,24 @@
+//Translation from Muller_Kahan.c
+//Should Verify
+//NOTE:  (fp(....)) causes a compiler error!
+//FAILS!  Heavily...
+
+procedure main() returns () {
+	var x0 : float(11 53);
+	var x1 : float(11 53);
+	var x2 : float(11 53);
+	var i : int;
+	
+	x0 := fp(11 11 53) / fp(2 11 53);
+	x1 := fp(61 11 53) / fp(11 11 53);
+	i := 0;
+	while (i < 100) {
+		x2 := fp(1130 11 53) - fp(3000 11 53) / x0;
+		x2 := fp(111 11 53) - x2 / x1;
+		x0 := x1;
+		x1 := x2;
+		i := i + 1;
+	}
+	
+	assert(x0 >= fp(99 11 53) && x0 <= fp(101 11 53));
+}
