float_test16.bpl
@@ -1,0 +1,8 @@
+//Translation from nan_double_false-unreach-call.c
+//Should return an error
+
+procedure main() returns () {
+	var x : float(11 53);
+	havoc x;
+	assert(x==x);
+}
