float_test17.bpl
@@ -1,0 +1,11 @@
+//Translation from nan_double_range_true-unreach-call.c
+//Should verify
+//Uggghhhh, should I add support for e?
+
+procedure main() returns () {
+	var x : float(11 53);
+	havoc x;
+	if (x >= fp(-100000000000000000000000000 11 53) && x <= fp(100000000000000000000000000 11 53)) {	
+		assert(x==x);
+	}
+}
