float_test19.bpl
@@ -1,0 +1,36 @@
+//Translation from flim_invariant.c
+//Should verify
+//Unary - unsupported float operations (on my end)...
+
+procedure main() returns () {
+	var X : float;
+	var Y : float;
+	var S : float;
+	var R : float;
+	var D : float;
+	var i : int;
+	
+	Y := fp(0);
+	
+	i := 0;
+	while (i < 100000) {
+		havoc X;
+		havoc D;
+		assume(X >= fp(-128) && X <= fp(128));
+		assume(D >= fp(0) && D <= fp(16));
+		
+		S := Y;
+		Y := X;
+		R := X - S;
+		if (R <= fp(0)-D) {
+			Y := S - D;
+		}
+		else if(R >= D) {
+			Y := S + D;
+		}
+		
+		assert(Y >= fp(-129) && Y <= fp(129));
+		
+		i := i + 1;
+	}
+}
