float_test2.bpl
@@ -1,5 +1,13 @@
-procedure F() returns () {
-	var x : float(11 53);
-	var y : float(11 53);
-	assert x == y;
+//Translation from addsub_float_exact.c
+//Should Verify
+procedure main() returns () {
+	var x : float;
+	var y : float;
+	var z : float;
+	var r : float;
+	x := fp(1000000);
+	y := x + fp(1);
+	z := x - fp(1);
+	r := y - z;
+	assert r == fp(2);
 }
