float_test3.bpl
@@ -1,3 +1,13 @@
- procedure F() returns () {
-	assert fp(5) == fp(5 8 23);
+//Translation from addsub_float_inexact.c
+//Should give an error
+procedure main() returns () {
+	var x : float;
+	var y : float;
+	var z : float;
+	var r : float;
+	x := fp(10000000);
+	y := x + fp(1);
+	z := x - fp(1);
+	r := y - z;
+	assert r == fp(0);
 }
