float_test8.bpl
@@ -1,3 +1,12 @@
-procedure F() returns () {
-	assert fp(-oo)==fp(-oo);
+//Translation from float_double.c
+//Should Verify
+//FAILS: I don't have this functionality yet...
+
+procedure main() returns () {
+	var x : float(11 53);
+	var y : float;
+	
+	x := fp(100000000000000000001 11 53);
+	y := x;
+	assert(x != y);
 }
